stuff

ByteBlockCacheSystem/ByteBetreeBlockCache.i.dfy
@@ -27,6 +27,7 @@ module ByteBetreeBlockCache refines AsyncDiskMachine {
   import opened DiskLayout
   import opened JournalRanges`Internal
   import opened SectorType
+  import opened JournalBytes
 
   type Constants = BBC.Constants
   type Variables = BBC.Variables
@@ -51,64 +52,6 @@ module ByteBetreeBlockCache refines AsyncDiskMachine {
     && 32 <= |sector|
     && |sector| <= BlockSize()
     && ValidCheckedBytes(sector)
-  }
-
-  // There's some complexity here because we have to deal with
-  // journal blocks.
-
-  function {:opaque} JournalRangeOfByteSeq(s: seq<byte>): Option<JournalRange>
-  {
-    if s == [] then
-      Some([])
-    else if |s| >= 4096 && D.ChecksumChecksOut(s[0..4096]) then (
-      var rest := JournalRangeOfByteSeq(s[4096..]);
-      if rest.Some? then (
-        Some([s[32..4096]] + rest.value)
-      ) else (
-        None
-      )
-    )
-    else (
-      None
-    )
-  }
-
-  lemma JournalRangeOfByteSeqAdditive(a: seq<byte>, b: seq<byte>)
-  requires JournalRangeOfByteSeq(a).Some?
-  requires JournalRangeOfByteSeq(b).Some?
-  ensures JournalRangeOfByteSeq(a + b).Some?
-  ensures JournalRangeOfByteSeq(a + b).value
-        == JournalRangeOfByteSeq(a).value
-         + JournalRangeOfByteSeq(b).value
-
-  lemma JournalRangeOfByteSeqGetI(a: seq<byte>, i: int)
-  requires JournalRangeOfByteSeq(a).Some?
-  requires 0 <= i
-  requires 4096*(i+1) <= |a|
-  ensures JournalRangeOfByteSeq(a[4096*i .. 4096*(i+1)]).Some?
-  ensures i < JournalRangeLen(JournalRangeOfByteSeq(a).value)
-  ensures JournalRangeOfByteSeq(a[4096*i .. 4096*(i+1)]).value
-      == JournalBlockGet(JournalRangeOfByteSeq(a).value, i)
-  {
-    reveal_JournalRangeOfByteSeq();
-    if i == 0 {
-      var c := a[4096*i .. 4096*(i+1)];
-      assert JournalRangeOfByteSeq(c[4096..]) == Some([]);
-      assert c[0..4096] == c;
-    } else {
-      var a' := a[4096..];
-      assert a[4096*i .. 4096*(i+1)] == a'[4096*(i-1) .. 4096*i];
-      JournalRangeOfByteSeqGetI(a', i-1);
-      var rest := JournalRangeOfByteSeq(a');
-      assert ([a[32..4096]] + rest.value)[i] == rest.value[i-1];
-      //assert JournalRangeOfByteSeq(a[4096*i .. 4096*(i+1)])
-      //    == JournalRangeOfByteSeq(a'[4096*(i-1) .. 4096*i]);
-    }
-  }
-
-  predicate ValidJournalBytes(bytes: seq<byte>)
-  {
-    && JournalRangeOfByteSeq(bytes).Some?
   }
 
   predicate ValidLocationAndBytes(loc: Location, bytes: seq<byte>)
