ByteBlockCacheSystem/JournalBytes.i.dfy
@@ -1,0 +1,64 @@
+include "../BlockCacheSystem/JournalRange.i.dfy"
+include "AsyncDiskModel.s.dfy"
+
+module JournalBytes {
+  import opened NativeTypes
+  import opened JournalRanges`Internal
+  import opened Options
+  import D = AsyncDisk
+
+  function {:opaque} JournalRangeOfByteSeq(s: seq<byte>): Option<JournalRange>
+  {
+    if s == [] then
+      Some([])
+    else if |s| >= 4096 && D.ChecksumChecksOut(s[0..4096]) then (
+      var rest := JournalRangeOfByteSeq(s[4096..]);
+      if rest.Some? then (
+        Some([s[32..4096]] + rest.value)
+      ) else (
+        None
+      )
+    )
+    else (
+      None
+    )
+  }
+
+  lemma JournalRangeOfByteSeqAdditive(a: seq<byte>, b: seq<byte>)
+  requires JournalRangeOfByteSeq(a).Some?
+  requires JournalRangeOfByteSeq(b).Some?
+  ensures JournalRangeOfByteSeq(a + b).Some?
+  ensures JournalRangeOfByteSeq(a + b).value
+        == JournalRangeOfByteSeq(a).value
+         + JournalRangeOfByteSeq(b).value
+
+  lemma JournalRangeOfByteSeqGetI(a: seq<byte>, i: int)
+  requires JournalRangeOfByteSeq(a).Some?
+  requires 0 <= i
+  requires 4096*(i+1) <= |a|
+  ensures JournalRangeOfByteSeq(a[4096*i .. 4096*(i+1)]).Some?
+  ensures i < JournalRangeLen(JournalRangeOfByteSeq(a).value)
+  ensures JournalRangeOfByteSeq(a[4096*i .. 4096*(i+1)]).value
+      == JournalBlockGet(JournalRangeOfByteSeq(a).value, i)
+  {
+    reveal_JournalRangeOfByteSeq();
+    if i == 0 {
+      var c := a[4096*i .. 4096*(i+1)];
+      assert JournalRangeOfByteSeq(c[4096..]) == Some([]);
+      assert c[0..4096] == c;
+    } else {
+      var a' := a[4096..];
+      assert a[4096*i .. 4096*(i+1)] == a'[4096*(i-1) .. 4096*i];
+      JournalRangeOfByteSeqGetI(a', i-1);
+      var rest := JournalRangeOfByteSeq(a');
+      assert ([a[32..4096]] + rest.value)[i] == rest.value[i-1];
+      //assert JournalRangeOfByteSeq(a[4096*i .. 4096*(i+1)])
+      //    == JournalRangeOfByteSeq(a'[4096*(i-1) .. 4096*i]);
+    }
+  }
+
+  predicate ValidJournalBytes(bytes: seq<byte>)
+  {
+    && JournalRangeOfByteSeq(bytes).Some?
+  }
+}
