Impl/JournalistModel.i.dfy
@@ -1,0 +1,77 @@
+include "../ByteBlockCacheSystem/JournalBytes.i.dfy"
+include "../BlockCacheSystem/DiskLayout.i.dfy"
+
+module JournalistModel {
+  import opened JournalRanges
+  import opened JournalBytes
+  import opened Journal
+  import opened DiskLayout
+  import opened NativeTypes
+  import opened Options
+
+  datatype JournalInfo = JournalInfo(
+    inMemoryJournalFrozen: seq<JournalEntry>,
+    inMemoryJournal: seq<JournalEntry>,
+    replayJournal: seq<JournalEntry>,
+
+    journalFrontRead: Option<JournalRange>,
+    journalBackRead: Option<JournalRange>
+  )
+
+  datatype JournalistModel = JournalistModel(
+    journalEntries: seq<JournalEntry>,
+    fStart: uint64,
+    fLen: uint64,
+    eStart: uint64,
+    eLen: uint64,
+
+    replayJournal: seq<JournalEntry>,
+    replayIdx: uint64,
+
+    journalFrontRead: Option<seq<byte>>,
+    journalBackRead: Option<seq<byte>>)
+
+  function method Len() : uint64 { 1048576 }
+
+  predicate WF(jm: JournalistModel)
+  {
+    && |jm.journalEntries| == Len() as int
+    && 0 <= jm.fStart < Len()
+    && 0 <= jm.fLen <= Len()
+    && 0 <= jm.eStart < Len()
+    && 0 <= jm.eLen <= Len()
+    && 0 <= jm.replayIdx as int <= |jm.replayJournal|
+    && (jm.journalFrontRead.Some? ==>
+        JournalRangeOfByteSeq(jm.journalFrontRead.value).Some?)
+    && (jm.journalBackRead.Some? ==>
+        JournalRangeOfByteSeq(jm.journalBackRead.value).Some?)
+  }
+
+  function cyclicSlice<T>(t: seq<T>, start: uint64, l: uint64) : seq<T>
+  requires 0 <= start as int < |t|
+  requires 0 <= l as int <= |t|
+  {
+    if start as int + l as int <= |t| then
+      t[start .. start + l]
+    else
+      t[start ..] + t[.. start + l - |t| as uint64]
+  }
+
+  function IJournalRead(j: Option<seq<byte>>) : Option<JournalRange>
+  requires j.Some? ==> JournalRangeOfByteSeq(j.value).Some?
+  {
+    if j.Some? then JournalRangeOfByteSeq(j.value) else None
+  }
+    
+  protected function I(jm: JournalistModel) : JournalInfo
+  requires WF(jm)
+  {
+    JournalInfo(
+      cyclicSlice(jm.journalEntries, jm.fStart, jm.fLen),
+      cyclicSlice(jm.journalEntries, jm.eStart, jm.eLen),
+      replayJournal[replayIdx..],
+      IJournalRead(jm.journalFrontRead),
+      IJournalRead(jm.journalBackRead)
+    )
+  }
+}
